compiler/backend/data_to_wordScript.sml
@@ -1314,9 +1314,9 @@ local val assign_quotation = `
         let header1 = Load addr1 in
         let k = dimindex(:'a) - shift(:'a) - c.len_size in
         let fakelen1 = Shift Lsr header1 (Nat k) in
-        let addr2 = real_addr c (adjust_var v1) in
-        let header2 = Load addr1 in
-        let fakelen2 = Shift Lsr header1 (Nat k) in            
+        let addr2 = real_addr c (adjust_var v2) in
+        let header2 = Load addr2 in
+        let fakelen2 = Shift Lsr header2 (Nat k) in            
         (list_Seq [
           Assign 1 (Op Add [addr1; Const bytes_in_word]);
           Assign 3 (Op Sub [fakelen1; Const (bytes_in_word-1w)]);
