compiler/backend/semantics/stackSemScript.sml
@@ -475,10 +475,10 @@ val evaluate_def = tDefine "evaluate" `
     case (get_var len s, get_var ptr s,get_var len2 s, get_var ptr2 s) of
     | SOME (Word w),SOME (Word w2),SOME (Word w3),SOME (Word w4) =>
          (case (read_bytearray w2 (w2n w) (mem_load_byte_aux s.memory s.mdomain s.be),
-                read_bytearray w2 (w2n w) (mem_load_byte_aux s.memory s.mdomain s.be)) of
+                read_bytearray w4 (w2n w3) (mem_load_byte_aux s.memory s.mdomain s.be)) of
           | SOME bytes,SOME bytes2 =>
               let (new_ffi,new_bytes) = call_FFI s.ffi ffi_index bytes bytes2 in
-              let new_m = write_bytearray w2 new_bytes s.memory s.mdomain s.be in
+              let new_m = write_bytearray w4 new_bytes s.memory s.mdomain s.be in
                 (NONE, s with <| memory := new_m ;
                                  regs := DRESTRICT s.regs s.ffi_save_regs;
                                  ffi := new_ffi |>)
